src/arch/x64/X64.Vale.Decls_i.fsti
@@ -1,5 +1,5 @@
 module X64.Vale.Decls_i
-module M = Memory_i_s
+module M = X64.Memory_i_s
 
 // This interface should hide all of Semantics_s.
 // (It should not refer to Semantics_s, directly or indirectly.)
@@ -55,20 +55,22 @@ unfold let va_operand_xmm = xmm
 (* Abbreviations *)
 unfold let get_reg (o:va_reg_operand) : reg = OReg?.r o
 //unfold let buffer_readable = M.buffer_readable
-unfold let buffer_readable (#t:M.typ) (h:mem) (b:M.buffer t) = M.buffer_readable #t h b
+unfold let buffer_readable (#t:M.typ) (h:M.mem) (b:M.buffer t) = M.buffer_readable #t h b
 //unfold let buffer_length = M.buffer_length
 unfold let buffer_length (#t:M.typ) (b:M.buffer t) = M.buffer_length #t b
-unfold let buffer64_as_seq (m:mem) (b:buffer64) : GTot (Seq.seq nat64) = M.buffer_as_seq m b
-unfold let buffer128_as_seq (m:mem) (b:buffer128) : GTot (Seq.seq quad32) = M.buffer_as_seq m b
-unfold let valid_src_addr (#t:M.typ) (m:mem) (b:M.buffer t) (i:int) : Type0 =
+unfold let buffer64_as_seq (m:M.mem) (b:M.buffer64) : GTot (Seq.seq nat64) = M.buffer_as_seq m b
+unfold let buffer128_as_seq (m:M.mem) (b:M.buffer128) : GTot (Seq.seq quad32) = M.buffer_as_seq m b
+unfold let valid_src_addr (#t:M.typ) (m:M.mem) (b:M.buffer t) (i:int) : Type0 =
   0 <= i /\ i < buffer_length b /\ buffer_readable m b
-unfold let valid_dst_addr (#t:M.typ) (m:mem) (b:M.buffer t) (i:int) : Type0 =
+unfold let valid_dst_addr (#t:M.typ) (m:M.mem) (b:M.buffer t) (i:int) : Type0 =
   0 <= i /\ i < buffer_length b /\ buffer_readable m b
-unfold let buffer64_read (b:buffer64) (i:int) (m:mem) : nat64 = M.buffer_read b i m
-unfold let buffer64_write (b:buffer64) (i:int) (v:nat64) (m:mem) : mem = M.buffer_write b i v m
-unfold let buffer128_read (b:buffer128) (i:int) (m:mem) : quad32 = M.buffer_read b i m
-unfold let buffer128_write (b:buffer128) (i:int) (v:quad32) (m:mem) : mem = M.buffer_write b i v m
-unfold let modifies_mem (s:M.loc) (h1 h2:mem) : GTot Type0 = M.modifies s h1 h2
+unfold let buffer64_read (b:M.buffer64) (i:int) (m:M.mem) : GTot nat64 = M.buffer_read b i m
+unfold let buffer64_write (b:M.buffer64) (i:int) (v:nat64) (m:M.mem) : GTot M.mem = 
+  if buffer_readable m b then m else M.buffer_write b i v m
+unfold let buffer128_read (b:M.buffer128) (i:int) (m:M.mem) : GTot quad32 = M.buffer_read b i m
+unfold let buffer128_write (b:M.buffer128) (i:int) (v:quad32) (m:M.mem) : GTot M.mem = 
+  if buffer_readable m b then m else M.buffer_write b i v m
+unfold let modifies_mem (s:M.loc) (h1 h2:M.mem) : GTot Type0 = M.modifies s h1 h2
 //unfold let loc_buffer = M.loc_buffer
 unfold let loc_buffer(#t:M.typ) (b:M.buffer t) = M.loc_buffer #t b
 unfold let locs_disjoint = M.locs_disjoint
@@ -110,23 +112,23 @@ unfold let va_opr_code_Mem (o:operand) (offset:int) : operand =
   | OReg r -> OMem (MReg r offset)
   | _ -> OConst 42
 
-let va_opr_lemma_Mem (s:va_state) (base:operand{OReg? base}) (offset:int) (b:buffer64) (index:int) : Lemma
+let va_opr_lemma_Mem (s:va_state) (base:operand{OReg? base}) (offset:int) (b:M.buffer64) (index:int) : Lemma
   (requires
     valid_src_addr s.mem b index /\
-    eval_operand base s + offset == buffer_addr b + 8 `op_Multiply` index
+    eval_operand base s + offset == M.buffer_addr b s.mem + 8 `op_Multiply` index
   )
   (ensures valid_operand (va_opr_code_Mem base offset) s)
   =
-  lemma_valid_mem64 b index s.mem
+  M.lemma_valid_mem64 b index s.mem
   
 
 (* Evaluation *)
-[@va_qattr] unfold let va_eval_opr64        (s:va_state) (o:va_operand)     : nat64 = eval_operand o s
-[@va_qattr] unfold let va_eval_dst_opr64    (s:va_state) (o:va_dst_operand) : nat64 = eval_operand o s
-[@va_qattr] unfold let va_eval_shift_amt64  (s:va_state) (o:va_shift_amt)   : nat64 = eval_operand o s
-[@va_qattr] unfold let va_eval_cmp_uint64   (s:va_state) (r:va_cmp)         : nat64 = eval_operand r s
-[@va_qattr] unfold let va_eval_reg64        (s:va_state) (r:va_register)    : nat64 = eval_reg r s
-[@va_qattr] unfold let va_eval_reg_opr64    (s:va_state) (o:va_operand)     : nat64 = eval_operand o s
+[@va_qattr] unfold let va_eval_opr64        (s:va_state) (o:va_operand)     : GTot nat64 = eval_operand o s
+[@va_qattr] unfold let va_eval_dst_opr64    (s:va_state) (o:va_dst_operand) : GTot nat64 = eval_operand o s
+[@va_qattr] unfold let va_eval_shift_amt64  (s:va_state) (o:va_shift_amt)   : GTot nat64 = eval_operand o s
+[@va_qattr] unfold let va_eval_cmp_uint64   (s:va_state) (r:va_cmp)         : GTot nat64 = eval_operand r s
+[@va_qattr] unfold let va_eval_reg64        (s:va_state) (r:va_register)    : GTot nat64 = eval_reg r s
+[@va_qattr] unfold let va_eval_reg_opr64    (s:va_state) (o:va_operand)     : GTot nat64 = eval_operand o s
 [@va_qattr] unfold let va_eval_xmm          (s:va_state) (x:xmm)            : quad32 = eval_xmm x s
 
 (* Predicates *)
@@ -146,11 +148,11 @@ let va_opr_lemma_Mem (s:va_state) (base:operand{OReg? base}) (offset:int) (b:buf
 [@va_qattr] unfold let va_get_flags (s:va_state) : int = s.flags
 [@va_qattr] unfold let va_get_reg (r:reg) (s:va_state) : nat64 = eval_reg r s
 [@va_qattr] unfold let va_get_xmm (x:xmm) (s:va_state) : quad32 = eval_xmm x s
-[@va_qattr] unfold let va_get_mem (s:va_state) : mem = s.mem
+[@va_qattr] unfold let va_get_mem (s:va_state) : M.mem = s.mem
 
 [@va_qattr] let va_upd_ok (ok:bool) (s:state) : state = { s with ok = ok }
 [@va_qattr] let va_upd_flags (flags:nat64) (s:state) : state = { s with flags = flags }
-[@va_qattr] let va_upd_mem (mem:mem) (s:state) : state = { s with mem = mem }
+[@va_qattr] let va_upd_mem (mem:M.mem) (s:state) : state = { s with mem = mem }
 [@va_qattr] let va_upd_reg (r:reg) (v:nat64) (s:state) : state = update_reg r v s
 [@va_qattr] let va_upd_xmm (x:xmm) (v:quad32) (s:state) : state = update_xmm x v s
 
@@ -272,43 +274,43 @@ let memModified (old_mem:mem) (new_mem:mem) (ptr:int) (num_bytes) =
 *)   
 
 (** Convenient memory-related functions **)
-let rec buffers_readable (h: mem) (l: list buffer64) : GTot Type0 (decreases l) =
+let rec buffers_readable (h: M.mem) (l: list M.buffer64) : GTot Type0 (decreases l) =
     match l with
     | [] -> True
     | b :: l'  -> buffer_readable h b /\ buffers_readable h l'
 
-unfold let modifies_buffer (b:buffer64) (h1 h2:mem) = modifies_mem (loc_buffer b) h1 h2
-unfold let modifies_buffer_2 (b1 b2:buffer64) (h1 h2:mem) =modifies_mem (M.loc_union (loc_buffer b1) (loc_buffer b2)) h1 h2
-unfold let modifies_buffer128 (b:buffer128) (h1 h2:mem) = modifies_mem (loc_buffer b) h1 h2
-unfold let modifies_buffer128_2 (b1 b2:buffer128) (h1 h2:mem) = modifies_mem (M.loc_union (loc_buffer b1) (loc_buffer b2)) h1 h2
+unfold let modifies_buffer (b:M.buffer64) (h1 h2:M.mem) = modifies_mem (loc_buffer b) h1 h2
+unfold let modifies_buffer_2 (b1 b2:M.buffer64) (h1 h2:M.mem) =modifies_mem (M.loc_union (loc_buffer b1) (loc_buffer b2)) h1 h2
+unfold let modifies_buffer128 (b:M.buffer128) (h1 h2:M.mem) = modifies_mem (loc_buffer b) h1 h2
+unfold let modifies_buffer128_2 (b1 b2:M.buffer128) (h1 h2:M.mem) = modifies_mem (M.loc_union (loc_buffer b1) (loc_buffer b2)) h1 h2
 
-let validSrcAddrs64 (m:mem) (addr:int) (b:buffer64) (len:int) =
+let validSrcAddrs64 (m:M.mem) (addr:int) (b:M.buffer64) (len:int) =
     buffer_readable m b /\
     len <= buffer_length b /\
-    buffer_addr b == addr
+    M.buffer_addr b m == addr
 
 unfold 
 let validDstAddrs64 = validSrcAddrs64
 
-let validSrcAddrs128 (m:mem) (addr:int) (b:buffer128) (len:int) =
+let validSrcAddrs128 (m:M.mem) (addr:int) (b:M.buffer128) (len:int) =
     buffer_readable m b /\
     len <= buffer_length b /\
-    buffer_addr b == addr
+    M.buffer_addr b m == addr
 
-let validDstAddrs128 (m:mem) (addr:int) (b:buffer128) (len:int) =
+let validDstAddrs128 (m:M.mem) (addr:int) (b:M.buffer128) (len:int) =
     buffer_readable m b /\
     len <= buffer_length b /\
-    buffer_addr b == addr
+    M.buffer_addr b m == addr
 
-let valid_stack_slots (m:mem) (rsp:int) (b:buffer64) (num_slots:int) =
+let valid_stack_slots (m:M.mem) (rsp:int) (b:M.buffer64) (num_slots:int) =
     buffer_readable m b /\
     num_slots <= buffer_length b /\
     (let open FStar.Mul in
-     rsp == buffer_addr b + 8 * num_slots /\
+     rsp == M.buffer_addr b m + 8 * num_slots /\
      0 <= rsp - 8 * num_slots /\ 
      rsp < pow2_64)
 
-let modifies_buffer_specific128 (b:buffer128) (h1 h2:mem) (start last:nat) : GTot Type0 =
+let modifies_buffer_specific128 (b:M.buffer128) (h1 h2:M.mem) (start last:nat) : GTot Type0 =
     modifies_buffer128 b h1 h2 /\
     // TODO: Consider replacing this with: modifies (loc_buffer (gsub_buffer b i len)) h1 h2
     (forall (i:nat) . {:pattern (Seq.index (M.buffer_as_seq h2 b) i)}
@@ -317,7 +319,7 @@ let modifies_buffer_specific128 (b:buffer128) (h1 h2:mem) (start last:nat) : GTo
                     ==> buffer128_read b i h1
                      == buffer128_read b i h2)
 
-let modifies_buffer_specific (b:buffer64) (h1 h2:mem) (start last:nat) : GTot Type0 =
+let modifies_buffer_specific (b:M.buffer64) (h1 h2:M.mem) (start last:nat) : GTot Type0 =
     modifies_buffer b h1 h2 /\
     // TODO: Consider replacing this with: modifies (loc_buffer (gsub_buffer b i len)) h1 h2
     (forall (i:nat) . {:pattern (Seq.index (M.buffer_as_seq h2 b) i)}
@@ -326,13 +328,13 @@ let modifies_buffer_specific (b:buffer64) (h1 h2:mem) (start last:nat) : GTot Ty
                     ==> buffer64_read b i h1
                      == buffer64_read b i h2)
 
-unfold let buffers_disjoint (b1 b2:buffer64) =
+unfold let buffers_disjoint (b1 b2:M.buffer64) =
     locs_disjoint [loc_buffer b1; loc_buffer b2]
 
-unfold let buffers_disjoint128 (b1 b2:buffer128) =
+unfold let buffers_disjoint128 (b1 b2:M.buffer128) =
     locs_disjoint [loc_buffer b1; loc_buffer b2]
 
-unfold let buffers3_disjoint128 (b1 b2 b3:buffer128) =
+unfold let buffers3_disjoint128 (b1 b2 b3:M.buffer128) =
     locs_disjoint [loc_buffer b1; loc_buffer b2; loc_buffer b3]
 
 val eval_code (c:va_code) (s0:va_state) (f0:va_fuel) (sN:va_state) : Type0
